\documentclass[11pt]{article}

\include{header}

\begin{document}
\homework{13}{7 October}

Recall the list induction principle to prove a proeprty for finite lists of type $a$.

\[\begin{array}{l}

[P([\,]) \wedge \\
\;\;\forall{}x::a.\,\forall xs::[a].\, P(xs) \Rightarrow P(x:xs) \\
\;\;\; \Rightarrow \forall{}ys::[a]. P(ys)
\end{array}\]

Thus, for a property $P$ of lists, to show that $\forall{}ys::[a].\; P(ys)$ it
is enough to show two things:
\[\begin{array}{rl}
{\bf{i.)}} & P([\,]) \\
{\bf{ii.)}} & \forall x::a.\,\forall{}xs::[a].\, P(xs) \Rightarrow P(x:xs)\\
\end{array}\]

Here are some definitions.
\[\begin{array}{l}

head (h:t) = h \\
head [\,] = \bot \\
\ \\
last [x] = x \\
last (h:t) = last \; t \\
last [\,] = \bot \\
\ \\
reverse [\,] = [\,]\\
reverse (h:t) = (reverse \; t ) ++ [h] \\
\ \\
map\; f\, [\,] = [\,] \\
map \; f \; (h:t) = (f\; h)\, :\, map \; f \; t \\
\ \\
(f\, .\, g)\; x = f\, (g\; x)\\

\end{array}\]


Prove the following by list induction.

\[\begin{array}{ll}
%1.) & \forall{}m \!:\![a].\; map \,(\backslash x \rightarrow x)\; m = m \\
1.) & \forall{}m \!:\![a].\; map \,(f\, .\; g)\, m = ((map\; f)\, .\, (map\; g))\; m\\
2.) & \forall{}m \!:\![a].\; head\, (reverse \; m) = last \; m \\
3.) & \forall{}m \!:\![a].\; last\, (reverse \; m) = head \; m
\end{array}
\]




\end{document}
% Local Variables:
% mode:latex
% comment-column:0
% comment-start: "% "
% compile-command: "pdflatex hw13b"
% fill-column:79
% End:




