\documentclass[11pt]{article}

\include{header}

\begin{document}
\homework{3}{5 September}

Prove the following.  You may use the methods taught by Cowles \&
Velleman (Givens and Goals) or use the sequent rules from the handout.

\goodbreak\noindent
\begin{enumerate}
%\item  $\vdash \neg\neg{}p \Rightarrow {}p$\\
% \item  $\vdash {}p  \Rightarrow \neg\neg{}p$\\
%\item  $\vdash \neg{}p  \Rightarrow (p\Rightarrow\bot)$\\
% \item  $\vdash (p\Rightarrow\bot) \Rightarrow \neg{}p $\\
%\item  $\vdash (p\wedge{}q) \Rightarrow (p\vee{}q)$\\
% \item  $\vdash ((p\wedge{}q) \vee r) \Rightarrow (r\vee{}q)$\\
% \item  $\vdash \neg(p \wedge q) \Rightarrow (\neg p \vee \neg q)$\\
%\item  $\vdash  (p \wedge (p \Rightarrow q)) \Rightarrow q$\\
% \item  $\vdash \neg(p \vee q) \Rightarrow (\neg p \wedge \neg q)$\\
% \item  $\vdash  p \vee \neg p $\\
% \item   $\vdash \neg (\bot \wedge (p_1 \wedge (p_2 \wedge (p_3 \wedge (p_4 \wedge (p_5 \wedge (p_6 \wedge (p_7 \wedge p_8))))))))$\\
%\item   $\vdash ((p \wedge q) \Rightarrow r) \Rightarrow ((p \Rightarrow r) \vee (q \Rightarrow r))$\\

\item{} \Sequent{}{(\exists{}x.(P(x)\vee R(x))) \Rightarrow ((\exists{}x.P(x)) \vee \exists{}x.R(x)) }\\

\item{} \Sequent{}{(\forall{}x.(P(x)\wedge R(x))) \Rightarrow ((\forall{}x.P(x)) \wedge \forall{}x.R(x)) }\\

\item{} \Sequent{}{\neg(\exists{}x.P(x)) \Rightarrow (\forall{}x.\neg{}P(x)) }\\

\item{} \Sequent{}{(S \Rightarrow \forall{}x.P(x)) \Rightarrow (\forall{}x. S \Rightarrow P(x)) }\\

% \item{} \Sequent{(\forall{}x.P(x)) \Rightarrow S}{\exists{}x.(P(x) \Rightarrow S)}\\


\end{enumerate}




\end{document}
% Local Variables:
% mode:latex
% comment-column:0
% comment-start: "\\> "
% comment-end: "\\\\ "
% compile-command: "pdflatex hw3h"
% fill-column:79
% End:




