\documentclass[11pt]{article}

\include{header}
\newcommand{\appenda}[2]{{\mathit{append}}\;{#1}\;{#2}}
\newcommand{\List}[1]{[{#1}]}
\newcommand{\definedAsM}{\stackrel{{\mathrm{def}}}{=}}
\newcommand{\base}{\goodbreak\noindent{}Base case:}
\newcommand{\indstep}{\goodbreak\noindent{}Induction Step:}
\newcommand{\cons}{:}
\newcommand{\dpair}[1]{{\langle\!\langle{{#1}}\rangle\!\rangle}}
\renewcommand{\nil}{[\,]}
\begin{document}
\homework{7}{25 September}


Recall the induction principle for finite lists.

\[\begin{array}{l}

[P([\,]) \wedge \\
\;\;\forall x::a.\, \forall xs::[a].\, P(xs) \Rightarrow P(x:xs)] \\
\;\;\; \Rightarrow \forall{}ys::[a]. P(ys)
\end{array}\]

Thus, for a property $P$ of lists, to show that $\forall{}xs::[a].\; P(xs)$
it is enough to show two things:
\[\begin{array}{rl}
{\bf{i.)}} & P([\,]) \\
{\bf{ii.)}} & \forall x::a.\, \forall xs::[a].\,\; P(xs) \Rightarrow P(x:xs)\\
\end{array}\]

Here are the definitions of some list functions.
\[\begin{array}{l}

length\, [\,] = 0  \\
length\, (x:xs) = 1 + length\, xs \\
\ \\
append\, [\,] ys = ys \\
append\, (x:xs) ys = x: (append\, xs ys) \\
\ \\
map\; f\, [\,] = [\,] \\
map \; f \; (x:xs) = (f\; x)\, :\, map \; f \; xs \\
\ \\
(f\, .\, g)\; x = f\, (g\; x)\\

\end{array}\]



Definition of the append function shows directly that $\nil$
is a left identity for $\appenda{}{}$, is it a right identity as well? The
following theorem establishes this fact.

\begin{theorem}[Nil right identity for $\appenda{}{}$]
\label{thm:nil_right}
\index{right identity@Nil for $\appenda{}{}$}
\[\forall{}ys::\List{a}.\;\, \appenda{ys}{\nil} = ys\]
\ \\{\bf{Proof:}}
By list induction on $ys$.  The property $P$ of $ys$ is given as:
\[P(ys)\definedAsM \appenda{ys}{\nil} = ys\]

\base{} Show $P(\nil)$, {\em{i.e.}} that $\appenda{\nil}{\nil}=\nil$.  This
follows immediately from the definition of append.

\indstep{} Assume $P(xs)$ (the induction hypothesis) and show $P(x\cons{}xs)$
for arbitrary $x$ of type $a$ and arbitrary $xs$ of type $\List{A}$.  The induction
hypothesis is:
\[\appenda{xs}{\nil} = xs\]
We must show $\appenda{(x\cons{}xs)}{\nil} = (x\cons{}xs)$.  Starting with the left side
of the equality we get the following:
\[\appenda{(x\cons{xs})}{\nil} \stackrel{\dpair{{\mathit{def. of}} \appenda{}{}}}{=} x\cons(\appenda{xs}{\nil}) \stackrel{\dpair{ind. hyp.}}{=} x\cons{}xs\]
So the induction step holds and the proof is complete.  \qed
\end{theorem}



\begin{exercise}

Prove the following by list induction.

\[\begin{array}{ll}
1.) & \forall{}ys \!::\![a].\; length\, (map \,f\, ys) = length\, ys\\
2.) & \forall{}ys\!::\![a].\;\forall{}xs \!::\![a].\; length\, (append\,\, xs\,ys) = (length\,\; xs) + (length\,\; ys) \\
\end{array}
\]

For the second proof - choose an arbitrary lets $ys$ of type $[a]$ and then do list induction on $xs$.

\end{exercise}
\end{document}
% Local Variables:
% mode:latex
% comment-column:0
% comment-start: "% "
% compile-command: "pdflatex hw7e"
% fill-column:79
% End:




